Day 5: Tweaks & More Theorems

Gaea/Peano/Rules.lean
@@ -38,85 +38,96 @@ class NatZero {P : Sort u} {T : Type v}
   (L : Logic P) (N : IsNat P T) (Z : Zero T) :=
   (natZero : L |- nat (0 : T))
 
-namespace NatZero
+def natZero {P : Sort u} {T : Type v} 
+  {L : Logic P} [N : IsNat P T] [Z : Zero T] [C : NatZero L N Z] := C.natZero
+
 def nat0 {P : Sort u} {T : Type v} 
   {L : Logic P} [N : IsNat P T] [Z : Zero T] [C : NatZero L N Z] := C.natZero
-end NatZero
-
-export NatZero (natZero nat0)
 
 -- Axiom 2
 class EqNatRefl {P : Sort u} {T : Sort v} 
-  (L : Logic P) (N : IsNat P T) (Eq : LEq P T) :=
+  (L : Logic P) (N : IsNat P T) (Q : LEq P T) :=
   (eqNatRefl : (x : T) -> (L |- nat x) -> (L |- x = x))
 
-export EqNatRefl (eqNatRefl)
+def eqNatRefl {P : Sort u} {T : Sort v} 
+  {L : Logic P} [N : IsNat P T] [Q : LEq P T] [C : EqNatRefl L N Q]
+  {x : T} := C.eqNatRefl x
 
 -- Axiom 3
 class EqNatSymm {P : Sort u} {T : Sort v} 
-  (L : Logic P) (N : IsNat P T) (Eq : LEq P T) :=
+  (L : Logic P) (N : IsNat P T) (Q : LEq P T) :=
   (eqNatSymm : (x y : T) -> (L |- nat x) -> (L |- nat y) ->
     (L |- x = y) -> (L |- y = x))
 
-export EqNatSymm (eqNatSymm)
+def eqNatSymm {P : Sort u} {T : Sort v} 
+  {L : Logic P} [N : IsNat P T] [Q : LEq P T] [C : EqNatSymm L N Q]
+  {x y : T} := C.eqNatSymm x y
 
 -- Axiom 4
 class EqNatTrans {P : Sort u} {T : Sort v} 
-  (L : Logic P) (N : IsNat P T) (Eq : LEq P T) :=
+  (L : Logic P) (N : IsNat P T) (Q : LEq P T) :=
   (eqNatTrans : (x y z : T) -> (L |- nat x) -> (L |- nat y) -> (L |- nat z) -> 
     (L |- x = y) -> (L |- y = z) -> (L |- x = z))
 
-export EqNatTrans (eqNatTrans)
+def eqNatTrans {P : Sort u} {T : Sort v} 
+  {L : Logic P} [N : IsNat P T] [Q : LEq P T] [C : EqNatTrans L N Q]
+  {x y z : T} := C.eqNatTrans x y z
 
 -- Axiom 5
 class NatEqNat {P : Sort u} {T : Sort v} 
-  (L : Logic P) (N : IsNat P T) (Eq : LEq P T) :=
+  (L : Logic P) (N : IsNat P T) (Q : LEq P T) :=
   (natEqNat : (a b : T) -> (L |- nat b) -> (L |- a = b) -> (L |- nat a))
 
-namespace NatEqNat
-def natEq {P : Sort u} {T : Sort v} 
-{L : Logic P} [N : IsNat P T] [Eq : LEq P T] [C : NatEqNat L N Eq] 
-{a b : T} : (L |- nat b) -> (L |- a = b) -> (L |- nat a) := C.natEqNat a b
-end NatEqNat
+def natEqNat {P : Sort u} {T : Sort v} 
+  {L : Logic P} [N : IsNat P T] [Q : LEq P T] [C : NatEqNat L N Q] 
+  {a b : T} := C.natEqNat a b
 
-export NatEqNat (natEqNat natEq)
+def natEq {P : Sort u} {T : Sort v} 
+  {L : Logic P} [N : IsNat P T] [Q : LEq P T] [C : NatEqNat L N Q] 
+  {a b : T} := C.natEqNat a b
 
 -- Axiom 6
 class NatSuccNat {P : Sort u} {T : Sort v} 
   (L : Logic P) (N : IsNat P T) (Su : Succ T) :=
   (natSuccNat : (n : T) -> (L |- nat n) -> (L |- nat (S n)))
 
-namespace NatSuccNat
+def natSuccNat {P : Sort u} {T : Sort v} 
+{L : Logic P} [N : IsNat P T] [Su : Succ T] [C : NatSuccNat L N Su] 
+{n : T} := C.natSuccNat n
+
 def natS {P : Sort u} {T : Sort v} 
 {L : Logic P} [N : IsNat P T] [Su : Succ T] [C : NatSuccNat L N Su] 
-{n : T} : (L |- nat n) -> (L |- nat (S n)) := C.natSuccNat n
-end NatSuccNat
-
-export NatSuccNat (natSuccNat natS)
+{n : T} := C.natSuccNat n
 
 -- Axiom 7a
 class EqNatToEqSucc {P : Sort u} {T : Sort v} 
-  (L : Logic P) (N : IsNat P T) (Eq : LEq P T) (Su : Succ T) :=
+  (L : Logic P) (N : IsNat P T) (Q : LEq P T) (Su : Succ T) :=
   (eqNatToEqSucc : (m n : T) -> (L |- nat m) -> (L |- nat n) -> 
     (L |- m = n) -> (L |- S m = S n))
 
-export EqNatToEqSucc (eqNatToEqSucc)
+def eqNatToEqSucc {P : Sort u} {T : Sort v} 
+  {L : Logic P} [N : IsNat P T] [Q : LEq P T] [Su : Succ T]
+  [C : EqNatToEqSucc L N Q Su] {m n : T} := C.eqNatToEqSucc m n
 
 -- Axiom 7b
 class EqSuccToEqNat {P : Sort u} {T : Sort v} 
-  (L : Logic P) (N : IsNat P T) (Eq : LEq P T) (Su : Succ T) :=
+  (L : Logic P) (N : IsNat P T) (Q : LEq P T) (Su : Succ T) :=
   (eqSuccToEqNat : (m n : T) -> (L |- nat m) -> (L |- nat n) -> 
     (L |- S m = S n) -> (L |- m = n))
 
-export EqSuccToEqNat (eqSuccToEqNat)
+def eqSuccToEqNat {P : Sort u} {T : Sort v} 
+  {L : Logic P} [N : IsNat P T] [Q : LEq P T] [Su : Succ T]
+  [C : EqSuccToEqNat L N Q Su] {m n : T} := C.eqSuccToEqNat
 
 -- Axiom 8
 class SuccNatEqZeroFalse {P : Sort u} {T : Type v} 
-  (L : Logic P) (N : IsNat P T) (Eq : LEq P T) (Z : Zero T) (Su : Succ T) [False P] :=
+  (L : Logic P) (N : Nat P T) (Q : LEq P T) (F : LFalse P) :=
   (succNatEqZeroFalse : (m n : T) -> (L |- nat m) -> (L |- nat n) -> 
     (L |- S n = 0) -> (L |- false))
 
-export SuccNatEqZeroFalse (succNatEqZeroFalse)
+def succNatEqZeroFalse {P : Sort u} {T : Type v} 
+  {L : Logic P} [N : Nat P T] [Q : LEq P T] [F : LFalse P]
+  [C : SuccNatEqZeroFalse L N Q F] := C.succNatEqZeroFalse
 
 -- Axiom 9
 -- Induction over predicates
@@ -127,8 +138,8 @@ class NatInduction {P : Sort u} {T : Type v}
     ((n : T) -> (L |- nat n) -> (L |- f n) -> (L |- f (S n))) ->
     ((n : T) -> (L |- nat n) -> (L |- f n)))
 
-def natInduction {P : Sort u} {T : Type v} 
-  {L : Logic P} [N : Nat P T] [I : NatInduction L N] := I.natInduction
+def natInduction {P : Sort u} {T : Type v} {L : Logic P} 
+  [N : Nat P T] [I : NatInduction L N] {f : T -> P} := I.natInduction f
 
 -- Axiom 9 (Alt)
 -- Induction over schemas
@@ -147,30 +158,41 @@ def natInduction' {P : Sort u} {T : Type v}
 
 -- Axiom 1
 class AddNatZeroEqNat {P : Sort u} {T : Type v} 
-  (L : Logic P) (N : IsNat P T) (Eq : LEq P T) (A : Add T) (Z : Zero T) :=
+  (L : Logic P) (N : IsNat P T) (Q : LEq P T) (A : Add T) (Z : Zero T) :=
   (addNatZeroEqNat : (a : T) -> (L |- nat a) -> (L |- a + 0 = a))
 
-namespace AddNatZeroEqNat
-def An0_eq_n {P : Sort u} {T : Type v} 
-  {L : Logic P} [N : IsNat P T] [Eq : LEq P T] [A : Add T] [Z : Zero T] 
-  [C : AddNatZeroEqNat L N Eq A Z] {a : T} := C.addNatZeroEqNat a
-end AddNatZeroEqNat
-
-export AddNatZeroEqNat (addNatZeroEqNat An0_eq_n)
+def addNatZeroEqNat {P : Sort u} {T : Type v} 
+  {L : Logic P} [N : IsNat P T] [Q : LEq P T] [A : Add T] [Z : Zero T] 
+  [C : AddNatZeroEqNat L N Q A Z] {a : T} := C.addNatZeroEqNat a
 
 -- Axiom 2
 class AddNatSuccEqSucc {P : Sort u} {T : Type v} 
-  (L : Logic P) (N : IsNat P T) (Eq : LEq P T) (A : Add T) (Su : Succ T) := 
+  (L : Logic P) (N : IsNat P T) (Q : LEq P T) (A : Add T) (Su : Succ T) := 
   (addNatSuccEqSucc : (a b : T) -> (L |- nat a) -> (L |- nat b) -> 
     (L |- a + S b = S (a + b)))
 
-namespace AddNatSuccEqSucc
-def AmSn_eq_SAmn {P : Sort u} {T : Type v} 
-  {L : Logic P} [N : IsNat P T] [Eq : LEq P T] [A : Add T] [Su : Succ T]
-  [C : AddNatSuccEqSucc L N Eq A Su] {a b : T} := C.addNatSuccEqSucc a b
-end AddNatSuccEqSucc
+def addNatSuccEqSucc {P : Sort u} {T : Type v} 
+  {L : Logic P} [N : IsNat P T] [Q : LEq P T] [A : Add T] [Su : Succ T]
+  [C : AddNatSuccEqSucc L N Q A Su] {a b : T} := C.addNatSuccEqSucc a b
 
-export AddNatSuccEqSucc (addNatSuccEqSucc AmSn_eq_SAmn)
+-- Axiom 1 Commuted
+class AddZeroNatEqNat {P : Sort u} {T : Type v} 
+  (L : Logic P) (N : IsNat P T) (Q : LEq P T) (A : Add T) (Z : Zero T) :=
+  (addZeroNatEqNat : (a : T) -> (L |- nat a) -> (L |- 0 + a = a))
+
+def addZeroNatEqNat {P : Sort u} {T : Type v} 
+  {L : Logic P} [N : IsNat P T] [Q : LEq P T] [A : Add T] [Z : Zero T] 
+  [C : AddZeroNatEqNat L N Q A Z] {a : T} := C.addZeroNatEqNat a
+
+-- Axiom 2 Commuted
+class AddSuccNatEqSucc {P : Sort u} {T : Type v} 
+  (L : Logic P) (N : IsNat P T) (Q : LEq P T) (A : Add T) (Su : Succ T) := 
+  (addSuccNatEqSucc : (a b : T) -> (L |- nat a) -> (L |- nat b) -> 
+    (L |- S a + b = S (a + b)))
+
+def addSuccNatEqSucc {P : Sort u} {T : Type v} 
+  {L : Logic P} [N : IsNat P T] [Q : LEq P T] [A : Add T] [Su : Succ T]
+  [C : AddSuccNatEqSucc L N Q A Su] {a b : T} := C.addSuccNatEqSucc a b
 
 --------------------------------------------------------------------------------
 -- Multiplication Rules
@@ -178,14 +200,14 @@ export AddNatSuccEqSucc (addNatSuccEqSucc AmSn_eq_SAmn)
 
 -- Axiom 1
 class MulNatZeroEqZero {P : Sort u} {T : Type v} 
-  (L : Logic P) (N : IsNat P T) (Eq : LEq P T) (M : Mul T) (Z : Zero T)  :=
+  (L : Logic P) (N : IsNat P T) (Q : LEq P T) (M : Mul T) (Z : Zero T)  :=
   (mulNatZeroEqZero : (a : T) -> (L |- nat a) -> (L |- a * 0 = 0))
 
 export MulNatZeroEqZero (mulNatZeroEqZero)
 
 -- Axiom 2
 class MulNatSuccEqAddMul {P : Sort u} {T : Type v} 
-  (L : Logic P) (N : IsNat P T) (Eq : LEq P T) (M : Mul T) (A : Add T) (Su : Succ T) := 
+  (L : Logic P) (N : IsNat P T) (Q : LEq P T) (M : Mul T) (A : Add T) (Su : Succ T) := 
   (mulNatSuccEqAddMul : (a b : T) -> (L |- nat a) -> (L |- nat b) -> 
     (L |- a + S b = a + S (a * b)))
 
