Gaea/Peano/Theorems.lean
@@ -14,7 +14,7 @@ namespace Gaea.Peano
 -- General Theorems
 --------------------------------------------------------------------------------
 
-theorem natCases 
+def natCases 
 {P : Sort u} {T : Type v} {L : Logic P} [N : Nat P T] [NatInduction L N]
 : (f : T -> P) -> 
   (L |- f 0) -> ((n : T) -> (L |- nat n) -> (L |- f (S n))) -> 
@@ -23,52 +23,130 @@ theorem natCases
   intro f f0 fS n Nn
   have ih : (n : T) -> (L |- nat n) -> (L |- f n) -> (L |- f (S n)) := 
     fun n Nn fn => fS n Nn
-  exact natInduction f f0 ih n Nn
+  exact natInduction f0 ih n Nn
+
+class EqNatLeftEuc {P : Sort u} {T : Type v} 
+  (L : Logic P) (N : IsNat P T) (Q : LEq P T) :=
+  (eqNatLeftEuc : (a b c : T) -> 
+    (L |- nat a) -> (L |- nat b) -> (L |- nat c) -> 
+    (L |- b = a) -> (L |- c = a) -> (L |- b = c))
+
+def eqNatLeftEuc {P : Sort u} {T : Type v} 
+  {L : Logic P} [N : IsNat P T] [Q : LEq P T]
+  [C : EqNatLeftEuc L N Q] {a b c : T} := C.eqNatLeftEuc a b c 
+
+def eqNatLeftEuc_proof {P : Sort u} {T : Type v} {L : Logic P}
+[N : IsNat P T] [Q : LEq P T] [EqNatSymm L N Q] [EqNatTrans L N Q]
+: (a b c : T) -> 
+    (L |- nat a) -> (L |- nat b) -> (L |- nat c) -> 
+    (L |- b = a) -> (L |- c = a) -> (L |- b = c)
+:= by
+  intro a b c Na Nb Nc Qba Qca
+  have Qac := eqNatSymm Nc Na Qca
+  exact eqNatTrans Nb Na Nc Qba Qac
+
+instance eqNatLeftEuc_inst {P : Sort u} {T : Type v} {L : Logic P}
+  [N : IsNat P T] [Q : LEq P T] [EqNatSymm L N Q] [EqNatTrans L N Q]
+  : EqNatLeftEuc L N Q := {eqNatLeftEuc := eqNatLeftEuc_proof}
 
 --------------------------------------------------------------------------------
--- Addition Theorems
+-- Theorems related to Peano Addition being closed over the Naturals
 --------------------------------------------------------------------------------
 
-theorem addZeroEqZero 
-{P : Sort u} {T : Type v} {L : Logic P}
-[Q : LEq P T] [A : Add T] [Z : Zero T] [N : IsNat P T]
-[NatZero L N Z] [AddNatZeroEqNat L N Q A Z]
-: L |- 0 + 0 = (0 : T) 
-:= An0_eq_n nat0
+class NatAddNatZero {P : Sort u} {T : Type v} 
+  (L : Logic P) (N : IsNat P T) (A : Add T) (Z : Zero T) :=
+  (natAddNatZero : (a : T) -> (L |- nat a) -> (L |- nat (a + 0)))
 
-theorem natAddNatZero
+def natAddNatZero {P : Sort u} {T : Type v} 
+  {L : Logic P} [N : IsNat P T] [A : Add T] [Z : Zero T]
+  [C : NatAddNatZero L N A Z] {a : T} := C.natAddNatZero a
+
+def natAddNatZero_proof
 {P : Sort u} {T : Type v} {L : Logic P}
-[Q : LEq P T] [A : Add T] [Z : Zero T] [N : IsNat P T] 
+[N : IsNat P T] [Q : LEq P T] [A : Add T] [Z : Zero T]  
 [NatEqNat L N Q] [AddNatZeroEqNat L N Q A Z]
 : (a : T) -> (L |- nat a) -> (L |- nat (a + 0))
-:= by intro a Na; apply natEq Na; exact An0_eq_n Na
+:= by intro a Na; apply natEq Na; exact addNatZeroEqNat Na
 
--- Uses standard (predicate) induction
-theorem natAddNat_induct {P : Sort u} {T : Type v} {L : Logic P}
+instance natAddNatZero_inst 
+  {P : Sort u} {T : Type v} {L : Logic P}
+  [N : IsNat P T] [Q : LEq P T] [A : Add T] [Z : Zero T]  
+  [NatEqNat L N Q] [AddNatZeroEqNat L N Q A Z] : NatAddNatZero L N A Z 
+  := {natAddNatZero := natAddNatZero_proof}
+
+class NatAddZeroNat {P : Sort u} {T : Type v} 
+  (L : Logic P) (N : IsNat P T) (A : Add T) (Z : Zero T) :=
+  (natAddZeroNat : (a : T) -> (L |- nat a) -> (L |- nat (0 + a)))
+
+def natAddZeroNat {P : Sort u} {T : Type v} 
+  {L : Logic P} [N : IsNat P T] [A : Add T] [Z : Zero T]
+  [C : NatAddZeroNat L N A Z] {a : T} := C.natAddZeroNat a 
+
+def natAddZeroNat_proof
+{P : Sort u} {T : Type v} {L : Logic P}
+[N : IsNat P T] [Q : LEq P T] [A : Add T] [Z : Zero T]  
+[NatEqNat L N Q] [AddZeroNatEqNat L N Q A Z]
+: (a : T) -> (L |- nat a) -> (L |- nat (0 + a))
+:= by intro a Na; apply natEq Na; exact addZeroNatEqNat Na
+
+instance natAddZeroNat_inst 
+  {P : Sort u} {T : Type v} {L : Logic P}
+  [N : IsNat P T] [Q : LEq P T] [A : Add T] [Z : Zero T]  
+  [NatEqNat L N Q] [AddZeroNatEqNat L N Q A Z] : NatAddZeroNat L N A Z 
+  := {natAddZeroNat := natAddZeroNat_proof}
+
+-- Proofs related to Peano Addition being closed over the Naturals
+
+class NatAddNat {P : Sort u} {T : Type v}
+  (L : Logic P) (N : IsNat P T) (A : Add T) :=
+  (natAddNat : (a b : T) -> (L |- nat a) -> (L |- nat b) -> (L |- nat (a + b)))
+
+def natAddNat {P : Sort u} {T : Type v}
+  {L : Logic P} [N : IsNat P T] [A : Add T] [C : NatAddNat L N A]
+  {a b : T} := C.natAddNat a b
+
+def natAdd {P : Sort u} {T : Type v}
+  {L : Logic P} [N : IsNat P T] [A : Add T] [C : NatAddNat L N A]
+  {a b : T} := C.natAddNat a b
+
+instance natAddNatZero_spec {P : Sort u} {T : Type v}
+  {L : Logic P} [N : IsNat P T] [A : Add T] [Z : Zero T] [NatZero L N Z]
+  [C : NatAddNat L N A] : NatAddNatZero L N A Z 
+  := {natAddNatZero := fun a Na => C.natAddNat a 0 Na nat0 }
+
+instance natAddZeroNat_spec {P : Sort u} {T : Type v}
+  {L : Logic P} [N : IsNat P T] [A : Add T] [Z : Zero T] [NatZero L N Z]
+  [C : NatAddNat L N A] : NatAddZeroNat L N A Z 
+  := {natAddZeroNat := fun a Na => C.natAddNat 0 a nat0 Na }
+
+-- Uses standard (predicate) induction 
+def natAddNat_induct {P : Sort u} {T : Type v} {L : Logic P}
 [N : Nat P T] [Q : LEq P T] [A : PAdd L N Q] [Fa : MForall L T] [If : MIf L]
 [NatEqNat L N.toIsNat Q] [NatSuccNat L N.toIsNat N.toSucc] [NatInduction L N]
 : (b : T) -> (L |- nat b) -> (L |- forall (a : T) => nat a -> nat (a + b))
 := by
-  intro n Nn
-  apply natInduction 
-    (fun b => forall (a : T) => nat a -> nat (a + b))
-  exact forallNatIntro natAddNatZero
-  -- Induction
+  refine natInduction ?f0 ?fS
+  apply forallNatIntro; intro a Na 
+  exact natAddNatZero Na
   intro a Na p_Nn_to_NAna
   apply forallNatIntro; intro b Nb
-  have AbSa_eq_SAba := AmSn_eq_SAmn Nb Na
+  have AbSa_eq_SAba := addNatSuccEqSucc Nb Na
   have NAba := forallNatElim p_Nn_to_NAna Nb 
   exact natEq (natS NAba) AbSa_eq_SAba
-  exact Nn
 
-theorem natAddNat {P : Sort u} {T : Type v} {L : Logic P} 
+def natAddNat_proof {P : Sort u} {T : Type v} {L : Logic P} 
 [N : Nat P T] [Q : LEq P T] [A : PAdd L N Q] [Fa : MForall L T] [If : MIf L]
 [NatEqNat L N.toIsNat Q] [NatSuccNat L N.toIsNat N.toSucc] [NatInduction L N]
 : (a b : T) -> (L |- nat a) -> (L |- nat b) -> (L |- nat (a + b))
 := fun a b Na Nb => forallNatElim (natAddNat_induct b Nb) Na
 
+instance natAddNat_inst {P : Sort u} {T : Type v} {L : Logic P} 
+  [N : Nat P T] [Q : LEq P T] [A : PAdd L N Q] [Fa : MForall L T] [If : MIf L]
+  [NatEqNat L N.toIsNat Q] [NatSuccNat L N.toIsNat N.toSucc] [NatInduction L N]
+  : NatAddNat L N.toIsNat A.toAdd := {natAddNat := natAddNat_proof}
+
 -- Uses schema induction
-theorem natAddNat'
+def natAddNat_schema_proof
 {P : Sort u} {T : Type v} {L : Logic.{u,w} P}
 [N : Nat P T] [Q : LEq P T]  [A : PAdd L N Q]
 [NatEqNat L N.toIsNat Q] [NatSuccNat L N.toIsNat N.toSucc] 
@@ -80,13 +158,231 @@ theorem natAddNat'
     (fun (b : T) => (a : T) -> (L |- nat a) -> (L |- nat (a + b)))
   -- Base
   intro a Na
-  exact natAddNatZero a Na
+  exact natAddNatZero Na
   -- Induction
   intro a Na ih b Nb
   have NAba := ih b Nb 
-  have AbSa_eq_SAba := AmSn_eq_SAmn Nb Na
+  have AbSa_eq_SAba := addNatSuccEqSucc Nb Na
   have NSAba := natS NAba
   exact natEq NSAba AbSa_eq_SAba
   exact Nn; exact Nm
+
+instance natAddNat_schema_inst 
+  {P : Sort u} {T : Type v} {L : Logic.{u,w} P}
+  [N : Nat P T] [Q : LEq P T]  [A : PAdd L N Q]
+  [NatEqNat L N.toIsNat Q] [NatSuccNat L N.toIsNat N.toSucc] 
+  [NatInduction'.{u,v,(imax (v+1) w)} L N]
+  : NatAddNat L N.toIsNat A.toAdd := {natAddNat := natAddNat_schema_proof}
+
+--------------------------------------------------------------------------------
+-- Theorems related to Peano Addition being commutative
+--------------------------------------------------------------------------------
+
+-- 9 + 9 = 9
+
+def addZeroEqZero 
+{P : Sort u} {T : Type v} {L : Logic P}
+[Q : LEq P T] [A : Add T] [Z : Zero T] 
+[N : IsNat P T] [NatZero L N Z] [AddNatZeroEqNat L N Q A Z]
+: L |- 0 + 0 = (0 : T) 
+:= addNatZeroEqNat nat0
+
+-- 0 + a = 0
+
+def addZeroNatEqNat_proof
+{P : Sort u} {T : Type v} {L : Logic P} 
+[N : Nat P T] [Q : LEq P T] [A : PAdd L N Q] 
+[NatZero L N.toIsNat N.toZero] 
+[NatSuccNat L N.toIsNat N.toSucc]
+[EqNatTrans L N.toIsNat Q] 
+[EqNatToEqSucc L N.toIsNat Q N.toSucc]  
+[NatInduction L N]
+[NatAddNat L N.toIsNat A.toAdd] 
+: (a : T) -> (L |- nat a) -> (L |- 0 + a = a)
+:= by
+  refine natInduction addZeroEqZero ?fS
+  case fS => 
+    intro a Na A0a_eq_a
+    have NSa := natS Na
+    have NA0a := natAdd nat0 Na
+    have A0Sa_eq_SA0a := addNatSuccEqSucc nat0 Na
+    have AS0a_eq_Sa := eqNatToEqSucc NA0a Na A0a_eq_a
+    exact eqNatTrans (natAdd nat0 NSa) (natS NA0a) NSa 
+      A0Sa_eq_SA0a AS0a_eq_Sa
+
+instance addZeroNatEqNat_inst 
+  {P : Sort u} {T : Type v} {L : Logic P} 
+  [N : Nat P T] [Q : LEq P T] [A : PAdd L N Q] 
+  [NatZero L N.toIsNat N.toZero] [NatSuccNat L N.toIsNat N.toSucc]
+  [EqNatTrans L N.toIsNat Q] [EqNatToEqSucc L N.toIsNat Q N.toSucc]  
+  [NatInduction L N] [NatAddNat L N.toIsNat A.toAdd] 
+  : AddZeroNatEqNat L N.toIsNat Q A.toAdd N.toZero
+  := {addZeroNatEqNat := addZeroNatEqNat_proof}
+
+class AddNatZeroComm {P : Sort u} {T : Type v} 
+  (L : Logic P) (N : IsNat P T) (Q : LEq P T) (A : Add T) (Z : Zero T) :=
+  (addNatZeroComm : (a : T) -> (L |- nat a) -> (L |- a + 0 = 0 + a))
+
+def addNatZeroComm {P : Sort u} {T : Type v} 
+  {L : Logic P} [N : IsNat P T] [Q : LEq P T] [A : Add T] [Z : Zero T]
+  [C : AddNatZeroComm L N Q A Z] {a : T} := C.addNatZeroComm a
+
+-- 0 + a = a + 0
+
+def addNatZeroComm_proof
+{P : Sort u} {T : Type v} {L : Logic P} 
+[N : IsNat P T] [Q : LEq P T] [A : Add T] [Z : Zero T]
+[EqNatLeftEuc L N Q]
+[NatAddNatZero L N A Z]
+[NatAddZeroNat L N A Z]
+[AddNatZeroEqNat L N Q A Z]
+[AddZeroNatEqNat L N Q A Z]
+: (a : T) -> (L |- nat a) -> (L |- a + 0 = 0 + a)
+:= by
+  intro a Na; apply eqNatLeftEuc Na
+  exact natAddNatZero Na; exact natAddZeroNat Na
+  exact addNatZeroEqNat Na; exact addZeroNatEqNat Na 
+
+instance addNatZeroComm_inst 
+  {P : Sort u} {T : Type v} {L : Logic P} 
+  [N : IsNat P T] [Q : LEq P T] [A : Add T] [Z : Zero T]
+  [EqNatLeftEuc L N Q] [NatAddNatZero L N A Z] [NatAddZeroNat L N A Z]
+  [AddNatZeroEqNat L N Q A Z] [AddZeroNatEqNat L N Q A Z]
+  : AddNatZeroComm L N Q A Z 
+  := {addNatZeroComm := addNatZeroComm_proof}
+
+-- S a + b = S (a + b)
+
+def addSuccNatEqSucc_induct
+{P : Sort u} {T : Type v} {L : Logic P} 
+[N : Nat P T] [Q : LEq P T] [A : PAdd L N Q] [MForall L T] [MIf L]
+[NatZero L N.toIsNat N.toZero] 
+[NatSuccNat L N.toIsNat N.toSucc]
+[EqNatTrans L N.toIsNat Q]
+[EqNatLeftEuc L N.toIsNat Q]
+[EqNatToEqSucc L N.toIsNat Q N.toSucc]  
+[NatInduction L N]
+[NatAddNat L N.toIsNat A.toAdd] 
+: (b : T) -> (L |- nat b) -> (L |- forall a => nat a -> S a + b = S (a + b))
+:= by
+  refine natInduction ?f0 ?fS
+  case f0 => 
+    apply forallNatIntro; intro a Na
+    have NSa := natS Na; 
+    have NAa0 := natAdd Na nat0
+    apply eqNatLeftEuc NSa 
+      (natAdd NSa nat0) (natS NAa0)
+    exact addNatZeroEqNat (natS Na)
+    have Aa0_eq_a := addNatZeroEqNat Na
+    exact eqNatToEqSucc NAa0 Na Aa0_eq_a
+  case fS =>
+    intro b Nb p_ASnb_eq_Snb
+    apply forallNatIntro; intro a Na
+    have NSa := natS Na; have NSb := natS Nb
+    have NAaSb := natAdd Na NSb; have NSAaSb := natS NAaSb
+    have NASaSb := natAdd NSa NSb
+    have NAab := natAdd Na Nb; have NSAab := natS NAab; have NSSAab := natS NSAab
+    have NASab := natAdd NSa Nb; have NSASab := natS NASab; 
+    have ASab_eq_SAab := forallNatElim p_ASnb_eq_Snb Na
+    have AaSb_eq_SAab := addNatSuccEqSucc Na Nb
+    have ASaSb_eq_SASab := addNatSuccEqSucc NSa Nb
+    have SASab_eq_SSAab := eqNatToEqSucc NASab NSAab ASab_eq_SAab
+    have ASaSb_eq_SSAab := eqNatTrans NASaSb NSASab NSSAab 
+      ASaSb_eq_SASab SASab_eq_SSAab
+    have SAaSb_eq_SSAab := eqNatToEqSucc NAaSb NSAab AaSb_eq_SAab
+    exact eqNatLeftEuc NSSAab NASaSb NSAaSb ASaSb_eq_SSAab SAaSb_eq_SSAab
+
+def addSuccNatEqSucc_proof
+{P : Sort u} {T : Type v} {L : Logic P} 
+[N : Nat P T] [Q : LEq P T] [A : PAdd L N Q] [MForall L T] [MIf L]
+[NatInduction L N]
+[NatZero L N.toIsNat N.toZero] 
+[NatSuccNat L N.toIsNat N.toSucc]
+[EqNatTrans L N.toIsNat Q]
+[EqNatLeftEuc L N.toIsNat Q]
+[EqNatToEqSucc L N.toIsNat Q N.toSucc]  
+[NatAddNat L N.toIsNat A.toAdd] 
+: (a b : T) -> (L |- nat a) -> (L |- nat b) -> (L |- S a + b = S (a + b))
+:= by
+  intro a b Na Nb
+  have h := addSuccNatEqSucc_induct b Nb
+  exact forallNatElim h Na
+
+instance addSuccNatEqSucc_inst {P : Sort u} {T : Type v} {L : Logic P} 
+  [N : Nat P T] [Q : LEq P T] [A : PAdd L N Q] [MForall L T] [MIf L]
+  [NatZero L N.toIsNat N.toZero] [NatSuccNat L N.toIsNat N.toSucc]
+  [EqNatTrans L N.toIsNat Q] [EqNatLeftEuc L N.toIsNat Q]
+  [EqNatToEqSucc L N.toIsNat Q N.toSucc] [NatInduction L N]
+  [NatAddNat L N.toIsNat A.toAdd]
+  : AddSuccNatEqSucc L N.toIsNat Q A.toAdd N.toSucc
+  := {addSuccNatEqSucc := addSuccNatEqSucc_proof} 
+
+-- a + b = b + a
+
+class AddNatComm {P : Sort u} {T : Type v} 
+  (L : Logic P) (N : IsNat P T) (Q : LEq P T) (A : Add T) :=
+  (addNatComm : (a b : T) -> (L |- nat a) -> (L |- nat b) -> (L |- a + b = b + a))
+
+def addNatComm {P : Sort u} {T : Type v} 
+  {L : Logic P} [N : IsNat P T] [Q : LEq P T] [A : Add T]
+  [C : AddNatComm L N Q A] {a b : T} := C.addNatComm a b
+
+def addNatComm_induct {P : Sort u} {T : Type v} {L : Logic P} 
+[N : Nat P T] [Q : LEq P T] [A : PAdd L N Q] [Fa : MForall L T] [If : MIf L]
+[NatInduction L N]
+[NatZero L N.toIsNat N.toZero]
+[NatSuccNat L N.toIsNat N.toSucc]
+[EqNatLeftEuc L N.toIsNat Q]
+[EqNatToEqSucc L N.toIsNat Q N.toSucc]  
+[NatAddNat L N.toIsNat A.toAdd]
+[AddZeroNatEqNat L N.toIsNat Q A.toAdd N.toZero]
+[AddSuccNatEqSucc L N.toIsNat Q A.toAdd N.toSucc]
+: (b : T) -> (L |- nat b) -> (L |- forall a => nat a -> a + b = b + a) 
+:= by
+  refine natInduction ?f0 ?fS
+  case f0 =>
+    apply forallNatIntro; intro a Na
+    exact addNatZeroComm Na
+  case fS =>
+    intro b Nb p_Anb_comm
+    apply forallNatIntro; intro a Na
+    have NSb := natS Nb
+    have NAab := natAdd Na Nb; have NSAab := natS NAab;
+    have NAba := natAdd Nb Na; have NSAba := natS NAba
+    have NASba := natAdd NSb Na; have NASab := natAdd Na NSb
+    apply eqNatLeftEuc NSAab NASab NASba
+    exact addNatSuccEqSucc Na Nb
+    have Aab_comm := forallNatElim p_Anb_comm Na
+    have SAab_comm := eqNatToEqSucc NAab NAba Aab_comm
+    apply eqNatLeftEuc NSAba NASba NSAab
+    exact addSuccNatEqSucc Nb Na
+    have Aab_comm := forallNatElim p_Anb_comm Na
+    exact eqNatToEqSucc NAab NAba Aab_comm
+
+def addNatComm_proof {P : Sort u} {T : Type v} {L : Logic P} 
+[N : Nat P T] [Q : LEq P T] [A : PAdd L N Q] [Fa : MForall L T] [If : MIf L]
+[NatInduction L N]
+[NatZero L N.toIsNat N.toZero]
+[NatSuccNat L N.toIsNat N.toSucc]
+[EqNatTrans L N.toIsNat Q]
+[EqNatLeftEuc L N.toIsNat Q]
+[EqNatToEqSucc L N.toIsNat Q N.toSucc]  
+[NatAddNat L N.toIsNat A.toAdd]
+: (a b : T) -> (L |- nat a) -> (L |- nat b) -> (L |- a + b = b + a) 
+:= by
+  intro a b Na Nb
+  have h := addNatComm_induct b Nb
+  exact forallNatElim h Na
+
+instance addNatComm_inst 
+  {P : Sort u} {T : Type v} {L : Logic P} 
+  [N : Nat P T] [Q : LEq P T] [A : PAdd L N Q] 
+  [Fa : MForall L T] [If : MIf L]
+  [NatInduction L N]
+  [NatZero L N.toIsNat N.toZero] [NatSuccNat L N.toIsNat N.toSucc]
+  [EqNatTrans L N.toIsNat Q] [EqNatLeftEuc L N.toIsNat Q] 
+  [EqNatToEqSucc L N.toIsNat Q N.toSucc] [NatAddNat L N.toIsNat A.toAdd]
+  : AddNatComm L N.toIsNat Q A.toAdd 
+  := {addNatComm := addNatComm_proof}
 
 end Gaea.Peano
