Gaea/Peano/Modules.lean
@@ -29,15 +29,9 @@ namespace PAdd
 def addNatZeroEqNat {P : Sort u} {T : Type v} 
   {L : Logic P} {N : Nat P T} {Eq : LEq P T} (A : PAdd L N Eq) 
   := A.toAddNatZeroEqNat.addNatZeroEqNat
-def An0_eq_n {P : Sort u} {T : Type v} 
-  {L : Logic P} [N : Nat P T] [Eq : LEq P T] (A : PAdd L N Eq) 
-  {a : T} := A.toAddNatZeroEqNat.addNatZeroEqNat a
 def addNatSuccEqSucc {P : Sort u} {T : Type v} 
   {L : Logic P} [N : Nat P T] [Eq : LEq P T] (A : PAdd L N Eq)
   := A.toAddNatSuccEqSucc.addNatSuccEqSucc
-def AmSn_eq_SAmn {P : Sort u} {T : Type v} 
-  {L : Logic P} [N : Nat P T] [Eq : LEq P T] (A : PAdd L N Eq)
-  {a b : T} := A.toAddNatSuccEqSucc.addNatSuccEqSucc a b
 end PAdd
 
 end Gaea.Peano
